theories/examples/simple_program_specs.v
@@ -18,18 +18,21 @@ Section examples.
            ∗ r1 ↦ᵣ w1
            ∗ r2 ↦ᵣ inr (p, g, b, e, a)
            ∗ a ↦ₐ w2 }}}
-      (Executable : cap_lang.expr)
+      (Seq (Instr Executable) : cap_lang.expr)
       {{{ RET HaltedV; r1 ↦ᵣ w2 }}}.
   Proof.
     intros Hil Hih Hvpc Hpca1 Hvpc' [Hra Hwb] Hne.
     iIntros (φ) "(Hpc & Hpca & Hpca' & Hr1 & Hr2 & Ha) Hφ".
-    iApply (wp_load_success _ _ _ _ _ _ _ pc_a); eauto. iFrame.
-    iNext. iIntros "(Hpc & Hr1 & Hpc_a1)".
-    iApply (wp_halt _ _ _ _ pc_a1 with "[Hpc Hpca']"); eauto; first iFrame.
-    iNext. iIntros "[Hpc Hpca']".
+    iApply (wp_bind (fill [SeqCtx])).
+    iApply (wp_load_success _ _ _ _ _ _ _ pc_a with "[-Hpca' Hφ]"); eauto. iFrame.
+    iNext. iIntros "(Hpc & Hr1 & _ & _ & _) /=".
+    iApply wp_pure_step_later; eauto. iNext.z
+    iApply (wp_bind (fill [SeqCtx])). 
+    iApply (wp_halt _ _ _ _ _ pc_a1 with "[-Hr1 Hφ]"); eauto. iFrame. 
+    iNext. iIntros "[_ _] /=".
+    iApply wp_pure_step_later; eauto. iNext. 
+    iApply wp_value. 
     iApply "Hφ". iFrame. 
   Qed.
-
-  
 
 End examples. 
