theories/fundamental.v
@@ -4,7 +4,7 @@ From iris.program_logic Require Import weakestpre adequacy lifting.
 From stdpp Require Import base. 
 
 Section fundamental.
-  Context `{memG Σ, regG Σ, inG Σ frac.fracR}.
+  Context `{memG Σ, regG Σ, STSG Σ}.
   Notation D := ((leibnizC Word) -n> iProp Σ).
   Notation R := ((leibnizC Reg) -n> iProp Σ).
   Implicit Types w : (leibnizC Word).
@@ -33,140 +33,220 @@ Section fundamental.
     iSpecialize ("Hupdate" with "[Hmap]"); eauto.
   Qed.
 
-  Lemma key_non_dupl γ : ∀ q, own γ 1%Qp ∗ own γ q%Qp -∗ False.
+  Lemma extract_lookup_reg reg (r : RegName) :
+    ((∀ r0, ⌜is_Some (reg !! r0)⌝ ∧ (⌜r0 ≠ PC⌝ → (fixpoint interp1) (reg !r! r0))) →
+     ⌜is_Some (reg !! r)⌝)%I.
   Proof.
-    iIntros (q) "[H1 Hq]".
-    iDestruct (own_valid_2 γ with "[H1] [Hq]") as "%"; iFrame.
-    iPureIntro. rewrite frac.frac_op' in H2.
-    assert (((1 + q)%Qp ≤ 1%Qp)%Qc).
-      by apply frac.frac_valid'.
-    by apply (Qp_not_plus_q_ge_1 q). 
+    iIntros "Hreg". 
+    - iAssert (⌜is_Some (reg !! r)⌝ ∧ (⌜r ≠ PC⌝ → (fixpoint interp1) (reg !r! r)))%I
+        with "Hreg" as "Hreg". 
+      iDestruct ("Hreg") as "[Hr Hreg]". done. 
   Qed.
+
+  Lemma extract_valid_reg reg (r : RegName) :
+    r ≠ PC →
+    ((∀ r0, ⌜is_Some (reg !! r0)⌝ ∧ (⌜r0 ≠ PC⌝ → (fixpoint interp1) (reg !r! r0))) →
+     (fixpoint interp1) (reg !r! r))%I.
+  Proof.
+    iIntros (Hne) "Hreg".
+    iAssert (⌜is_Some (reg !! r)⌝ ∧ (⌜r ≠ PC⌝ → (fixpoint interp1) (reg !r! r)))%I
+                                             with "Hreg" as "[_ Hv]". 
+    iApply "Hv". iPureIntro. done. 
+  Qed. 
 
   Instance addr_inhabited: Inhabited Addr := populate (A 0%Z eq_refl). 
 
-  Lemma fundamental_RX_global b e γ (a : Addr) :
-    (read_cond b e Global γ interp -∗
-    ⟦ inr ((RX,Global),b,e,a) ⟧ₑ )%I. 
+  Lemma fundamental_RX b e g (a : Addr) ws :
+    (inv (logN .@ (b,e)) (read_only_cond b e ws interp) →
+    ⟦ inr ((RX,g),b,e,a) ⟧ₑ )%I. 
   Proof.
-    iIntros "#Hinv".
-    iIntros (r m) "Hreg".
+    iIntros "#Hinv /=".
+    iIntros (r m fs fr) "[Hreg [Hmreg Hsts]]".
     iExists _,_,_,_,_; iSplit; eauto; simpl.
-    iIntros "Hmreg /=".
-    iLöb as "IH". 
+    iLöb as "IH" forall (r a fs fr). 
     iApply (wp_bind (fill [SeqCtx])).
-    destruct (decide (isCorrectPC (inr ((RX,Global),b,e,a)))). 
+    destruct (decide (isCorrectPC (inr ((RX,g),b,e,a)))). 
     - (* Correct PC *)
       assert ((b <= a)%a ∧ (a <= e)%a) as Hbae.
       { eapply in_range_is_correctPC; eauto.
         unfold le_addr; omega. }
-      iInv (logN.@(b, e)) as (ws) "HregionHvalid" "Hcls".     
-      iDestruct (extract_from_region _ _ a with "HregionHvalid")
-       as (al w ah) "(Hal & Hah & Hregionl & Hvalidl & >Ha & Hva & Hregionh & Hvalidh)";
-        auto. 
-      iDestruct (extract_r (<[PC:=inr (RX, Global, b, e, a)]> r) PC
-                           (inr (RX, Global, b, e, a))
-                   with "[Hmreg]") as "[HPC HPCmap]";
-        first by apply (lookup_insert r PC). iFrame.
+      iInv (logN.@(b, e)) as "Hregion" "Hcls".      
+      iDestruct (extract_from_region _ _ a with "Hregion")
+        as (al w ah) "(Hal & Hah & Hregionl & Hvalidl & >Ha & #Hva & Hregionh & Hvalidh)";
+        auto.
+      iDestruct ((big_sepM_delete _ _ PC) with "Hmreg") as "[HPC Hmap]"; 
+        first apply (lookup_insert _ _ (inr (RX, g, b, e, a))). 
       destruct (cap_lang.decode w) eqn:Hi. (* proof by cases on each instruction *)
       + admit. (* Jmp *)
       + admit. (* Jnz *)
       + admit. (* Mov *)
       + (* Load *)
-        (* these come from the reg interp relation *)
-        iAssert (∃ w, dst ↦ᵣ w)%I as (wdst) "Hdst"; [admit|].
-        iAssert (∃ w, src ↦ᵣ w)%I as (wsrc) "Hsrc"; [admit|].
-        destruct wsrc eqn:Hsrc; [admit|].
-        destruct c. do 3 destruct p.
-        iAssert (∃ w, a0 ↦ₐ w)%I as (wa0) "Ha0"; [admit|].
-        
-        iApply (wp_load_success with "[HPC Hdst Hsrc Ha Ha0]"); eauto.
-        * admit.
-        * admit.
-        * admit.
-        * iFrame.
-        * iNext. iIntros "(HPC & Hdst & Ha) /=".
-          iApply (wp_wand with "[HPC Hreg HPCmap]").
-          { iApply wp_pure_step_later; eauto. iNext.
-            iApply ("IH" with "Hreg").
-            iSpecialize ("HPCmap" with "HPC"). rewrite insert_insert. iFrame. 
-          } iAssert (∀ v : val cap_lang,
-                        (λ _ : valC cap_lang, ∃ r0 : Reg, registers_mapsto r0) v
-                                -∗ ∃ r0 : Reg, registers_mapsto r0)%I as "Htrivial".
-          { iIntros (_) "Hreg". iFrame. } iFrame. 
-          iApply "Hcls". iNext.
-          iExists (ws). iApply (extract_from_region _ _ a); auto. 
-          iExists al, w, ah. iFrame.
-      + admit. (* Store *)
-      + admit. (* Lt *)
-      + admit. (* Add *)
-      + admit. (* Sub *)
-      + admit. (* Lea *)
-      + admit. (* Restrict *)
-      + admit. (* Subseg *)
-      + admit. (* IsPtr *)
-      + admit. (* GetL *)
-      + admit. (* GetP *)
-      + admit. (* GetB *)
-      + admit. (* GetE *)
-      + admit. (* GetA *)
-      + admit. (* Fail *)
-      + admit. (* Halt *)   
-    - (* Incorrect PC *) admit.
-  Admitted. 
+        (* TODO: destruct between success and fail, and different versions of the rule *)
+        destruct (decide (PC = dst)),(decide (PC = src)); simplify_eq. 
+        * (* Load PC PC ==> fail *)
+          iApply (wp_load_fail3 with "[HPC Ha]"); eauto; iFrame. 
+          iNext. iIntros "[HPC Ha] /=".
+          iApply wp_pure_step_later; auto.
+          iApply wp_value.
+          iDestruct (extract_from_region _ _ a with
+               "[Hal Hah Hregionl Hvalidl Hregionh Hvalidh Ha]") as "Hregion"; eauto.
+          { iExists al,w,ah. iFrame. iExact "Hva". }
+          iDestruct ((big_sepM_delete _ _ PC) with "[HPC Hmap]") as "Hmap /=".
+          apply lookup_insert. rewrite delete_insert_delete. iFrame.
+          rewrite insert_insert.
+          iExists (<[PC:=w]> r),fs,fr. iFrame.
+          iAssert (⌜related_sts fs fs fr fr⌝)%I as "#Hrefl". 
+          { iPureIntro. apply related_sts_refl. }
+          iFrame "#". iApply "Hcls". iNext. iFrame. 
+        * (* Load PC src ==> success if src ↦ inr, fail o/w *)
+          iDestruct (extract_lookup_reg r src with "Hreg") as "%".
+          destruct H2 as [wsrc Hsomesrc]. 
+          assert ((delete PC r !! src) = Some wsrc) as Hsomesrc'.
+          { rewrite -Hsomesrc. apply (lookup_delete_ne r PC src). eauto. }
+          rewrite delete_insert_delete.
+          iDestruct ((big_sepM_delete _ _ src) with "Hmap") as "[Hsrc Hmap]"; eauto.
+          destruct wsrc.
+          { (* src ↦ inl z ==> fail *)
+            iApply (wp_load_fail2 with "[HPC Ha Hsrc]"); eauto; iFrame.
+            iNext. iIntros "[HPC [Ha Hsrc]] /=".
+            iApply wp_pure_step_later; auto. iApply wp_value.
+            iDestruct (extract_from_region _ _ a with
+                 "[Hal Hah Hregionl Hvalidl Hregionh Hvalidh Ha]") as "Hregion"; eauto.
+            { iExists al,w,ah. iFrame. iExact "Hva". }
+            iDestruct ((big_sepM_delete _ _ src) with "[Hsrc Hmap]") as "Hmap /=".
+            apply lookup_insert. rewrite delete_insert_delete. iFrame.
+            rewrite -delete_insert_ne; auto.
+            iDestruct ((big_sepM_delete _ _ PC) with "[HPC Hmap]") as "Hmap /=".
+            apply lookup_insert. rewrite delete_insert_delete. iFrame.
+            iExists _,fs,fr. iFrame.
+            iAssert (⌜related_sts fs fs fr fr⌝)%I as "#Hrefl". 
+            { iPureIntro. apply related_sts_refl. }
+            iFrame "#". iApply "Hcls". iNext. iFrame. 
+          } 
+          (* src ↦ inr c ==> need to open invariant *)
+          destruct c. do 3 destruct p.
+          (* if p is not ra or a0 is not within bounds: fail *)
+          destruct (decide ((readAllowed p && withinBounds ((p,l),a2,a1,a0)) = false)).
+          { (* Capability fail *)
+            iApply (wp_load_fail1 with "[HPC Ha Hsrc]"); eauto.
+            - split; eauto. apply andb_false_iff. eauto.
+            - iFrame.
+            - iNext. iIntros "[HPC [Ha Hsrc]] /=".
+              iApply wp_pure_step_later; auto.
+              iApply wp_value.
+              iDestruct (extract_from_region _ _ a with
+                 "[Hal Hah Hregionl Hvalidl Hregionh Hvalidh Ha]") as "Hregion"; eauto.
+            { iExists al,w,ah. iFrame. iExact "Hva". }
+            iDestruct ((big_sepM_delete _ _ src) with "[Hsrc Hmap]") as "Hmap /=".
+            apply lookup_insert. rewrite delete_insert_delete. iFrame.
+            rewrite -delete_insert_ne; auto.
+            iDestruct ((big_sepM_delete _ _ PC) with "[HPC Hmap]") as "Hmap /=".
+            apply lookup_insert. rewrite delete_insert_delete. iFrame.
+            iExists _,fs,fr. iFrame.
+            iAssert (⌜related_sts fs fs fr fr⌝)%I as "#Hrefl". 
+            { iPureIntro. apply related_sts_refl. }
+            iFrame "#". iApply "Hcls". iNext. iFrame. 
+          }
+          (* readAllowed p && withinBounds ((p,l),a2,a1,a0) *)
+          apply (not_false_is_true (_ && _)),Is_true_eq_left,andb_prop_elim in n0
+            as [Hra Hwb]. apply andb_prop_elim in Hwb as [Hle Hge]. 
+          (* get validity of capability in src from Hreg *)
+          iDestruct (extract_valid_reg r src with "Hreg") as "#Hvsrc"; auto.
+          rewrite /RegLocate Hsomesrc.
+          iDestruct (read_allowed_inv with "Hvsrc") as "Hconds"; eauto. 
+          iDestruct "Hconds" as "[#Hro|#[Hrw|Hrwl]]".
+          (* each condition is similar, but with some subtle differences *)
+          { iDestruct "Hro" as (ws0) "Hinv0".
+            (* open the invariant to access a0 ↦ₐ _ *)
+            iInv (logN.@(a2, a1)) as "Hro_cond" "Hcls'";[admit|].
+            iDestruct (extract_from_region _ _ a0 with "Hro_cond")
+            as (a0l w0 a0h)
+            "(Ha0l & Ha0h & Hregion0l & Hvalid0l & >Ha0 & #Hva0 & Hregion0h & Hvalid0h)";
+              first (split; by apply Z.leb_le,Is_true_eq_true).
+            (* if w0 is a Z, load crashes *)
+            destruct w0.
+            { iApply (wp_load_fail5 with "[HPC Ha Hsrc Ha0]"); eauto.
+              - split; apply Is_true_eq_true; eauto.
+                apply andb_prop_intro. split; [apply Hle|apply Hge].
+              - iFrame.
+              - iNext. iIntros "[HPC [Ha [Hsrc Ha0]]] /=".
+                iApply wp_pure_step_later; auto.
+                iApply wp_value.
+                iDestruct (extract_from_region _ _ a with
+                  "[Hal Hah Hregionl Hvalidl Hregionh Hvalidh Ha]") as "Hregion"; eauto.
+                { iExists al,w,ah. iFrame. iExact "Hva". }
+                iDestruct ((big_sepM_delete _ _ src) with "[Hsrc Hmap]") as "Hmap /=".
+                apply lookup_insert. rewrite delete_insert_delete. iFrame.
+                rewrite -delete_insert_ne; auto.
+                iDestruct ((big_sepM_delete _ _ PC) with "[HPC Hmap]") as "Hmap /=".
+                apply lookup_insert. rewrite delete_insert_delete. iFrame.
+                iExists _,fs,fr. iFrame.
+                iAssert (⌜related_sts fs fs fr fr⌝)%I as "#Hrefl". 
+                { iPureIntro. apply related_sts_refl. }
+                iFrame "#". iApply "Hcls". iFrame. iApply "Hcls'". iNext.
+                iApply (extract_from_region _ _ a0);
+                  first (split; by apply Z.leb_le,Is_true_eq_true).
+                iFrame. iExists a0l, (inl z), a0h. iFrame. iExact "Hva0". 
+            }
+            destruct c,p0,p0,p0. 
+            destruct ((a3 + 1)%a) eqn:Ha0.
+            2: { (* If src points to top address, load crashes *)
+              iApply (wp_load_fail4 with "[HPC Hsrc Ha Ha0]"); eauto. 
+              - split; apply Is_true_eq_true; eauto.
+                apply andb_prop_intro. split; [apply Hle|apply Hge].
+              - iFrame.
+              - iNext. iIntros "[HPC [Ha [Hsrc Ha0]]] /=".
+                iApply wp_pure_step_later; auto.
+                iApply wp_value.
+                iDestruct (extract_from_region _ _ a with
+                  "[Hal Hah Hregionl Hvalidl Hregionh Hvalidh Ha]") as "Hregion"; eauto.
+                { iExists al,w,ah. iFrame. iExact "Hva". }
+                iDestruct ((big_sepM_delete _ _ src) with "[Hsrc Hmap]") as "Hmap /=".
+                apply lookup_insert. rewrite delete_insert_delete. iFrame.
+                rewrite -delete_insert_ne; auto.
+                iDestruct ((big_sepM_delete _ _ PC) with "[HPC Hmap]") as "Hmap /=".
+                apply lookup_insert. rewrite delete_insert_delete. iFrame.
+                iExists _,fs,fr. iFrame.
+                iAssert (⌜related_sts fs fs fr fr⌝)%I as "#Hrefl". 
+                { iPureIntro. apply related_sts_refl. }
+                iFrame "#". iApply "Hcls". iFrame. iApply "Hcls'". iNext.
+                iApply (extract_from_region _ _ a0);
+                  first (split; by apply Z.leb_le,Is_true_eq_true).
+                iFrame. iExists a0l, _, a0h. iFrame. iExact "Hva0". 
+            }
+            (* success load into PC *)
+            iApply (wp_load_success_PC with "[HPC Ha Hsrc Ha0]"); eauto.
+            - split; apply Is_true_eq_true; eauto.
+              apply andb_prop_intro. split; [apply Hle|apply Hge].
+            - iFrame.
+            - iNext. iIntros "[HPC [Ha [Hsrc Ha0]]] /=".
+              iApply wp_pure_step_later; auto.
+              iDestruct (extract_from_region _ _ a with
+                "[Hal Hah Hregionl Hvalidl Hregionh Hvalidh Ha]") as "Hregion"; eauto.
+              { iExists al,w,ah. iFrame. iExact "Hva". }
+              iDestruct ((big_sepM_delete _ _ src) with "[Hsrc Hmap]") as "Hmap /=".
+              apply lookup_insert. rewrite delete_insert_delete. iFrame.
+              rewrite -delete_insert_ne; auto.
+              iDestruct ((big_sepM_delete _ _ PC) with "[HPC Hmap]") as "Hmap /=".
+              apply lookup_insert. rewrite delete_insert_delete. iFrame.
+              admit. 
+              (* iApply ("IH" with "[Hmap]"). *)
+              (* iFrame.  *)
+              (* rewrite /registers_mapsto. *)
 
-  Lemma fundamental_RX_local b e γ (a : Addr) :
-    (read_cond b e Local γ interp -∗
-    ⟦ inr ((RX,Local),b,e,a) ⟧ₑ )%I. 
-  Proof.
-    iIntros "#Hinv".
-    iIntros (r m) "Hreg".
-    iExists _,_,_,_,_; iSplit; eauto; simpl.
-    iExists γ. iIntros "Hkey Hmreg /=".
-    iLöb as "IH". 
-    iApply (wp_bind (fill [SeqCtx])).
-    destruct (decide (isCorrectPC (inr ((RX,Local),b,e,a)))). 
-    - (* Correct PC *)
-      iInv (logN.@(b, e)) as "[HregionHvalid | >Hkey']" "Hcls";
-        last by iDestruct (key_non_dupl γ with "[Hkey Hkey']") as "Hf"; iFrame.
-      iDestruct "HregionHvalid" as (ws) "HregionHvalid". 
-      iDestruct (extract_from_region _ _ a with "HregionHvalid")
-        as (w) "(Hregionl & Hvalidl & >Ha & Hva & Hregionh & Hvalidh)".
-      { admit. }
-      { admit. }
-      { admit. } (* a + -1 and a + 1 are some addresses *)
-      iDestruct (extract_r (<[PC:=inr (RX, Local, b, e, a)]> r) PC
-                           (inr (RX, Local, b, e, a))
-                   with "[Hmreg]") as "[HPC HPCmap]";
-        first by apply (lookup_insert r PC). iFrame.
-      destruct (cap_lang.decode w) eqn:Hi. (* proof by cases on each instruction *)
-      + admit. (* Jmp *)
-      + admit. (* Jnz *)
-      + admit. (* Mov *)
-      + (* Load *)
-        (* these come from the reg interp relation *)
-        iAssert (∃ w, dst ↦ᵣ w)%I as (wdst) "Hdst"; [admit|].
-        iAssert (∃ w, src ↦ᵣ w)%I as (wsrc) "Hsrc"; [admit|].
-        destruct wsrc eqn:Hsrc; [admit|].
-        destruct c. do 3 destruct p.
-        iAssert (∃ w, a0 ↦ₐ w)%I as (wa0) "Ha0"; [admit|].
-        
-        iApply (wp_load_success with "[HPC Hdst Hsrc Ha Ha0]"); eauto.
-        * admit.
-        * admit.
-        * admit.
-        * iFrame.
-        * iNext. iIntros "(HPC & Hdst & Ha) /=".
-          iApply (wp_wand with "[HPC Hreg HPCmap Hkey]").
-          { iApply wp_pure_step_later; eauto. iNext.
-            iApply ("IH" with "Hreg Hkey").
-            iSpecialize ("HPCmap" with "HPC"). rewrite insert_insert. iFrame. 
-          } iAssert (∀ v : val cap_lang,
-                        (λ _ : valC cap_lang, ∃ r0 : Reg, registers_mapsto r0) v
-                         -∗ ∃ r0 : Reg, registers_mapsto r0)%I as "Htrivial".
-          { iIntros (_) "Hreg". iFrame. } iFrame. 
-          iApply "Hcls". iNext. iLeft.
-          iExists (drop (region_size b a) ws). iFrame.
+              (* iExists _,fs,fr. iFrame. *)
+              (* iAssert (⌜related_sts fs fs fr fr⌝)%I as "#Hrefl".  *)
+              (* { iPureIntro. apply related_sts_refl. } *)
+              (* iFrame "#". iApply "Hcls". iFrame. iApply "Hcls'". iNext. *)
+              (* iApply (extract_from_region _ _ a0); *)
+              (*   first (split; by apply Z.leb_le,Is_true_eq_true). *)
+              (* iFrame. iExists a0l, _, a0h. iFrame. iExact "Hva0".  *)
+              
+          }
+          { admit. }
+          { admit. }
+        * (* Load dst PC *) admit.
+        * (* Load dst src *) admit. 
       + admit. (* Store *)
       + admit. (* Lt *)
       + admit. (* Add *)
@@ -185,20 +265,14 @@ Section fundamental.
     - (* Incorrect PC *) admit.
   Admitted. 
   
-  Theorem fundamental (perm : Perm) b e g γ (a : Addr) :
-    (⌜perm = RX⌝ ∧ read_cond b e g γ interp)%I ∨
-    (⌜perm = RWX⌝ ∧ read_cond b e g γ interp ∧
-     write_cond b e g γ interp (λne w, ⌜isLocalWord w = false⌝))%I ∨
-    (⌜perm = RWLX⌝ ∧ read_cond b e g γ interp ∧
-     write_cond b e g γ interp (λne w, True%I))%I -∗
+  Theorem fundamental (perm : Perm) b e g (a : Addr) :
+    (⌜perm = RX⌝ ∧ ∃ ws, (inv (logN .@ (b,e)) (read_only_cond b e ws interp)%I)) ∨
+    (⌜perm = RWX⌝ ∧ (inv (logN .@ (b,e)) (read_write_cond b e interp)%I)) ∨
+    (⌜perm = RWLX⌝ ∧ (inv (logN .@ (b,e)) (read_write_local_cond b e interp)%I)) -∗
     ⟦ inr ((perm,g),b,e,a) ⟧ₑ.
   Proof. 
-    iIntros "[#[-> Hinv] | [#(Hrwx & Hrc & Hwc) | #(Hwlx & Hrc & Hwc)]]".
-    - destruct g.
-      + (* Global *)
-          by iApply fundamental_RX_global. 
-      + (* Local *)
-          by iApply fundamental_RX_local. 
+    iIntros "[#[-> Hinv] | [#[-> Hinv] | #[-> Hinv]]]".
+    - iDestruct "Hinv" as (ws) "Hinv". by iApply fundamental_RX. 
     - (* read and write condition, non local *) admit. 
     - (* read and write condition, permit local *) admit. 
 Admitted. 
