theories/sts.v
@@ -1,0 +1,195 @@
+From iris.algebra Require Import auth agree gmap.
+From iris.base_logic Require Export invariants.
+From iris.proofmode Require Import tactics.
+Import uPred.
+
+
+(** The CMRA for the heap of STS.
+    We register the state and the transition relation. *)
+Definition sts_stateUR := authUR (gmapUR positive (exclR (leibnizC positive))).
+
+Definition sts_relUR :=
+  authUR (gmapUR positive (agreeR (leibnizC (positive → positive → Prop)))).
+
+Definition STS_states := gmap positive positive.
+Definition STS_rels := gmap positive (positive → positive → Prop).
+
+(** The CMRA for the thread pool. *)
+Class STSG Σ :=
+  { sts_state_inG :> inG Σ sts_stateUR;
+    sts_rel_inG :> inG Σ sts_relUR;
+    sts_state_name : gname;
+    sts_rel_name : gname; }.
+
+Section definitionsS.
+  Context `{STSG Σ} `{Countable A}.
+
+  Definition sts_state (i : positive) (x : A) : iProp Σ
+    := own (A := sts_stateUR) sts_state_name (◯ {[ i := Excl (encode x) ]}).
+
+  Definition convert_rel (R : A → A → Prop) : positive → positive → Prop :=
+    λ x y, ∃ a b, x = encode a ∧ y = encode b ∧ R a b.
+
+  Definition sts_rel (i : positive) (R : A → A → Prop) : iProp Σ :=
+    own (A := sts_relUR) sts_rel_name (◯ {[ i := to_agree (convert_rel R) ]}).
+
+  (* very weird bug!!!
+     Any two of these conjuncts are ok on their own but not all three!
+     But, it works with program!!!!!!!!!!! *)
+  Program Definition sts_full `{STSG Σ} (fs : STS_states) (fr : STS_rels) : iProp Σ
+    := (⌜dom (gset positive) fs = dom (gset positive) fr⌝
+        ∗ own (A := sts_stateUR) sts_state_name (● (Excl <$> fs))
+          ∗ own (A := sts_relUR) sts_rel_name (● (to_agree <$> fr)))%I.
+
+  Definition related_sts (fs gs : STS_states) (fr gr : STS_rels) : Prop :=
+    dom (gset positive) fs ⊆ dom (gset positive) gs ∧
+    dom (gset positive) fr ⊆ dom (gset positive) gr ∧
+    ∀ i x y r r', fs !! i = Some x → gs !! i = Some y →
+                  fr !! i = Some r → gr !! i = Some r' → r = r' ∧ rtc r x y.
+
+  Global Instance sts_rel_Persistent i R : Persistent (sts_rel i R).
+  Proof. apply _. Qed.
+
+  Global Instance sts_rel_Timeless i R : Timeless (sts_rel i R).
+  Proof. apply _. Qed.
+
+  Global Instance sts_state_Timeless i x : Timeless (sts_state i x).
+  Proof. apply _. Qed.
+
+  Global Instance sts_full_Timeless fs fr : Timeless (sts_full fs fr).
+  Proof. apply _. Qed.
+
+End definitionsS.
+
+Typeclasses Opaque sts_state sts_rel sts_full related_sts.
+
+Section STS.
+  Context `{STSG Σ} `{Countable A}.
+  Implicit Types x y : positive.
+  Implicit Types a b : A.
+  Implicit Types fs gs : STS_states.
+  Implicit Types fr gr : STS_rels.
+  Implicit Types R : A → A → Prop.
+  Implicit Types Rp : positive → positive → Prop.
+
+  Lemma related_sts_refl fs fr : related_sts fs fs fr fr.
+  Proof.
+    split; [|split]; trivial.
+    intros; simplify_eq; eauto using rtc_refl.
+  Qed.
+
+  Lemma related_sts_trans fs fr gs gr hs hr :
+    related_sts fs gs fr gr → related_sts gs hs gr hr → related_sts fs hs fr hr.
+  Proof.
+    intros [Hf1 [Hf2 Hf3]] [Hg1 [Hg2 Hg3]]; split; [|split]; try by etrans.
+    intros i x y r r' Hfs Hhs Hfr Hhr.
+    specialize (Hf1 i); specialize (Hf2 i);
+      revert Hf1 Hf2; rewrite !elem_of_dom; intros Hf1 Hf2.
+    destruct Hf1; eauto; destruct Hf2; eauto.
+    edestruct Hf3; eauto; edestruct Hg3; eauto; simplify_eq.
+    split; etrans; eauto.
+  Qed.
+
+  Lemma sts_full_rel fs fr i R :
+    sts_full fs fr -∗ sts_rel i R -∗ ⌜fr !! i = Some (convert_rel R)⌝.
+  Proof.
+    rewrite /sts_full /sts_rel.
+    iIntros "[% [_ H1]] H2".
+    iDestruct (own_valid_2 with "H1 H2") as %[HR Hv]%auth_valid_discrete;
+      iPureIntro.
+    specialize (Hv i).
+    revert HR; rewrite /= left_id singleton_included;
+      intros [z [Hz HR]]; revert HR; rewrite Some_included_total; intros HR.
+    rewrite lookup_fmap in Hz, Hv.
+    destruct (fr !! i) eqn:Heq; rewrite Heq /= in Hz, Hv; last by inversion Hz.
+    revert Hv; rewrite Hz; intros [u Hu]%to_agree_uninj.
+    revert HR; rewrite -Hu; intros HR%to_agree_included%leibniz_equiv;
+      simplify_eq.
+    inversion Hz as [? ? Hz'|]; simplify_eq.
+    revert Hz'; rewrite -Hu; intros Hz'%to_agree_inj%leibniz_equiv; simplify_eq.
+    by eauto.
+  Qed.
+
+  Lemma sts_full_state fs fr i a :
+    sts_full fs fr -∗ sts_state i a -∗ ⌜fs !! i = Some (encode a)⌝.
+  Proof.
+    rewrite /sts_full /sts_state.
+    iIntros "[% [H1 _]] H2".
+    iDestruct (own_valid_2 with "H1 H2") as %[HR Hv]%auth_valid_discrete;
+      iPureIntro.
+    specialize (Hv i).
+    revert HR; rewrite /= left_id singleton_included;
+      intros [z [Hz HR]].
+    rewrite lookup_fmap in Hz Hv.
+    destruct (fs !! i) eqn:Heq; rewrite Heq /= in Hz Hv; last by inversion Hz.
+    apply leibniz_equiv in Hz; simplify_eq.
+    apply Some_included_exclusive in HR; auto; last by typeclasses eauto.
+    apply leibniz_equiv in HR; simplify_eq; eauto.
+  Qed.
+
+  Lemma sts_alloc fs fr a R :
+    sts_full fs fr ==∗
+             ∃ i, sts_full (<[i := encode a ]>fs) (<[i := convert_rel R ]>fr)
+                  ∗ ⌜i ∉ dom (gset positive) fs⌝ ∗ ⌜i ∉ dom (gset positive) fr⌝
+                  ∗ sts_state i a ∗ sts_rel i R.
+  Proof.
+    rewrite /sts_full /sts_rel /sts_state.
+    iIntros "[Hd [H1 H2]]".
+    iDestruct "Hd" as %Hd.
+    iMod (own_update
+            (A := sts_stateUR)
+            _ _
+            (● (Excl <$>
+                <[fresh (dom (gset positive) fs) := encode a]> fs)
+            ⋅ ◯ {[fresh (dom (gset positive) fs) := Excl (encode a)]})
+            with "H1") as "[H1 Hs]".
+    { apply auth_update_alloc.
+      rewrite fmap_insert /=.
+      apply: alloc_singleton_local_update; last done.
+      apply (not_elem_of_dom (D := gset positive)).
+      rewrite dom_fmap.
+      apply is_fresh. }
+    iMod (own_update
+            (A := sts_relUR)
+            _ _
+            (● (to_agree <$>
+                <[fresh (dom (gset positive) fs) := convert_rel R]> fr)
+            ⋅ ◯ {[fresh (dom (gset positive) fs) := to_agree (convert_rel R)]})
+            with "H2") as "[H2 Hr]".
+    { apply auth_update_alloc.
+      rewrite fmap_insert /=.
+      apply: alloc_singleton_local_update; last done.
+      apply (not_elem_of_dom (D := gset positive)).
+      rewrite dom_fmap Hd.
+      apply is_fresh. }
+    iModIntro.
+    iExists _; iFrame.
+    repeat iSplit; iPureIntro;
+      rewrite ?dom_insert_L ?Hd; by try apply is_fresh.
+  Qed.
+
+  Lemma sts_update fs fr i a b :
+    sts_full fs fr -∗ sts_state i a ==∗
+    sts_full (<[i := encode b ]>fs) fr ∗ sts_state i b.
+  Proof.
+    iIntros "Hsf Hi".
+    iDestruct (sts_full_state with "Hsf Hi") as %Hfs.
+    rewrite /sts_full /sts_rel /sts_state.
+    iDestruct "Hsf" as "[Hd [H1 H2]]".
+    iDestruct "Hd" as %Hd.
+    iCombine "H1" "Hi" as "H1".
+    iMod (own_update (A := sts_stateUR)
+            _ _
+            (● (<[i := Excl (encode b)]> (Excl <$> fs))
+               ⋅ ◯ {[i := Excl (encode b)]})
+            with "H1") as "[H1 Hs]".
+    { apply auth_update.
+      apply: singleton_local_update; eauto.
+      rewrite lookup_fmap Hfs //=.
+      by apply exclusive_local_update. }
+    rewrite fmap_insert dom_insert_L subseteq_union_1_L;
+      first by iModIntro; iFrame.
+    apply elem_of_subseteq_singleton, elem_of_dom; eauto.
+  Qed.
+
+End STS.
